theta xor with super short soundness proof!

Clean/Gadgets/Keccak/ThetaXor.lean
@@ -3,77 +3,149 @@ import Clean.Types.U64
 import Clean.Gadgets.Xor.Xor64
 import Clean.Gadgets.Keccak.KeccakState
 import Clean.Gadgets.Rotation64.Rotation64
+import Clean.Gadgets.Keccak.Keccak
 
 namespace Gadgets.Keccak.ThetaXor
+
 variable {p : ℕ} [Fact p.Prime]
 variable [p_large_enough: Fact (p > 512)]
 
-open Provable (field field2 fields)
 open FieldUtils (mod_256 floordiv)
 open Xor (xor_u64)
-open Clean.Gadgets.Keccak256
+open Clean.Gadgets.Keccak256 (KeccakState KeccakState_is_normalized_iff)
 
 structure Inputs (F : Type) where
   state : KeccakState F
-  d : vec_provable U64 5 F
+  d : ProvableVector U64 5 F
 
-instance : ProvableType Inputs where
-  size := (ProvableType.size KeccakState) + (ProvableType.size (vec_provable U64 5))
-  to_elements s := ProvableType.to_elements s.state ++ ProvableType.to_elements s.d
-  from_elements v :=
-    let state : KeccakState _ := ProvableType.from_elements <| v.take (ProvableType.size KeccakState)
-    let d : vec_provable U64 5 _ := ProvableType.from_elements <| v.drop (ProvableType.size KeccakState)
-    ⟨state, d⟩
+instance : ProvableStruct Inputs where
+  components := [KeccakState, ProvableVector U64 5]
+  to_components := fun { state, d } => .cons state (.cons d .nil)
+  from_components := fun (.cons state (.cons d .nil)) => { state, d }
 
 
-@[reducible]
-def Outputs := KeccakState
-
-def theta_xor (inputs : Var Inputs (F p)) : Circuit (F p) (Var Outputs (F p)) := do
+def theta_xor (inputs : Var Inputs (F p)) : Circuit (F p) (Var KeccakState (F p)) := do
   let ⟨state, d⟩ := inputs
   return #v[
-    ←subcircuit Gadgets.Xor.circuit ⟨(state.get 0), (d.get 0)⟩,
-    ←subcircuit Gadgets.Xor.circuit ⟨(state.get 1), (d.get 0)⟩,
-    ←subcircuit Gadgets.Xor.circuit ⟨(state.get 2), (d.get 0)⟩,
-    ←subcircuit Gadgets.Xor.circuit ⟨(state.get 3), (d.get 0)⟩,
-    ←subcircuit Gadgets.Xor.circuit ⟨(state.get 4), (d.get 0)⟩,
-    ←subcircuit Gadgets.Xor.circuit ⟨(state.get 5), (d.get 1)⟩,
-    ←subcircuit Gadgets.Xor.circuit ⟨(state.get 6), (d.get 1)⟩,
-    ←subcircuit Gadgets.Xor.circuit ⟨(state.get 7), (d.get 1)⟩,
-    ←subcircuit Gadgets.Xor.circuit ⟨(state.get 8), (d.get 1)⟩,
-    ←subcircuit Gadgets.Xor.circuit ⟨(state.get 9), (d.get 1)⟩,
-    ←subcircuit Gadgets.Xor.circuit ⟨(state.get 10), (d.get 2)⟩,
-    ←subcircuit Gadgets.Xor.circuit ⟨(state.get 11), (d.get 2)⟩,
-    ←subcircuit Gadgets.Xor.circuit ⟨(state.get 12), (d.get 2)⟩,
-    ←subcircuit Gadgets.Xor.circuit ⟨(state.get 13), (d.get 2)⟩,
-    ←subcircuit Gadgets.Xor.circuit ⟨(state.get 14), (d.get 2)⟩,
-    ←subcircuit Gadgets.Xor.circuit ⟨(state.get 15), (d.get 3)⟩,
-    ←subcircuit Gadgets.Xor.circuit ⟨(state.get 16), (d.get 3)⟩,
-    ←subcircuit Gadgets.Xor.circuit ⟨(state.get 17), (d.get 3)⟩,
-    ←subcircuit Gadgets.Xor.circuit ⟨(state.get 18), (d.get 3)⟩,
-    ←subcircuit Gadgets.Xor.circuit ⟨(state.get 19), (d.get 3)⟩,
-    ←subcircuit Gadgets.Xor.circuit ⟨(state.get 20), (d.get 4)⟩,
-    ←subcircuit Gadgets.Xor.circuit ⟨(state.get 21), (d.get 4)⟩,
-    ←subcircuit Gadgets.Xor.circuit ⟨(state.get 22), (d.get 4)⟩,
-    ←subcircuit Gadgets.Xor.circuit ⟨(state.get 23), (d.get 4)⟩,
-    ←subcircuit Gadgets.Xor.circuit ⟨(state.get 24), (d.get 4)⟩
-   ]
+    ←subcircuit Gadgets.Xor.circuit ⟨state.get 0, d.get 0⟩,
+    ←subcircuit Gadgets.Xor.circuit ⟨state.get 1, d.get 0⟩,
+    ←subcircuit Gadgets.Xor.circuit ⟨state.get 2, d.get 0⟩,
+    ←subcircuit Gadgets.Xor.circuit ⟨state.get 3, d.get 0⟩,
+    ←subcircuit Gadgets.Xor.circuit ⟨state.get 4, d.get 0⟩,
+    ←subcircuit Gadgets.Xor.circuit ⟨state.get 5, d.get 1⟩,
+    ←subcircuit Gadgets.Xor.circuit ⟨state.get 6, d.get 1⟩,
+    ←subcircuit Gadgets.Xor.circuit ⟨state.get 7, d.get 1⟩,
+    ←subcircuit Gadgets.Xor.circuit ⟨state.get 8, d.get 1⟩,
+    ←subcircuit Gadgets.Xor.circuit ⟨state.get 9, d.get 1⟩,
+    ←subcircuit Gadgets.Xor.circuit ⟨state.get 10, d.get 2⟩,
+    ←subcircuit Gadgets.Xor.circuit ⟨state.get 11, d.get 2⟩,
+    ←subcircuit Gadgets.Xor.circuit ⟨state.get 12, d.get 2⟩,
+    ←subcircuit Gadgets.Xor.circuit ⟨state.get 13, d.get 2⟩,
+    ←subcircuit Gadgets.Xor.circuit ⟨state.get 14, d.get 2⟩,
+    ←subcircuit Gadgets.Xor.circuit ⟨state.get 15, d.get 3⟩,
+    ←subcircuit Gadgets.Xor.circuit ⟨state.get 16, d.get 3⟩,
+    ←subcircuit Gadgets.Xor.circuit ⟨state.get 17, d.get 3⟩,
+    ←subcircuit Gadgets.Xor.circuit ⟨state.get 18, d.get 3⟩,
+    ←subcircuit Gadgets.Xor.circuit ⟨state.get 19, d.get 3⟩,
+    ←subcircuit Gadgets.Xor.circuit ⟨state.get 20, d.get 4⟩,
+    ←subcircuit Gadgets.Xor.circuit ⟨state.get 21, d.get 4⟩,
+    ←subcircuit Gadgets.Xor.circuit ⟨state.get 22, d.get 4⟩,
+    ←subcircuit Gadgets.Xor.circuit ⟨state.get 23, d.get 4⟩,
+    ←subcircuit Gadgets.Xor.circuit ⟨state.get 24, d.get 4⟩
+  ]
 
-def assumptions (state : Inputs (F p)) : Prop :=
-  true
-
-def spec (state : Inputs (F p)) (out: Outputs (F p)) : Prop :=
-  true
-
-def circuit : FormalCircuit (F p) Inputs Outputs where
+instance elaborated : ElaboratedCircuit (F p) Inputs (Var KeccakState (F p)) where
   main := theta_xor
-  assumptions := assumptions
-  spec := spec
-  local_length _ := sorry
-  local_length_eq := sorry
-  output _ i0 := sorry
-  output_eq := sorry
+  local_length _ := 200
+  output _ i0 := #v[
+    var_from_offset U64 (i0),
+    var_from_offset U64 (i0 + 8),
+    var_from_offset U64 (i0 + 16),
+    var_from_offset U64 (i0 + 24),
+    var_from_offset U64 (i0 + 32),
+    var_from_offset U64 (i0 + 40),
+    var_from_offset U64 (i0 + 48),
+    var_from_offset U64 (i0 + 56),
+    var_from_offset U64 (i0 + 64),
+    var_from_offset U64 (i0 + 72),
+    var_from_offset U64 (i0 + 80),
+    var_from_offset U64 (i0 + 88),
+    var_from_offset U64 (i0 + 96),
+    var_from_offset U64 (i0 + 104),
+    var_from_offset U64 (i0 + 112),
+    var_from_offset U64 (i0 + 120),
+    var_from_offset U64 (i0 + 128),
+    var_from_offset U64 (i0 + 136),
+    var_from_offset U64 (i0 + 144),
+    var_from_offset U64 (i0 + 152),
+    var_from_offset U64 (i0 + 160),
+    var_from_offset U64 (i0 + 168),
+    var_from_offset U64 (i0 + 176),
+    var_from_offset U64 (i0 + 184),
+    var_from_offset U64 (i0 + 192)
+  ]
 
-  soundness := by sorry
-  completeness := by sorry
+def assumptions (inputs : Inputs (F p)) : Prop :=
+  let ⟨state, d⟩ := inputs
+  (∀ i : Fin 25, state[i].is_normalized) ∧ (∀ i : Fin 5, d[i].is_normalized)
+
+def spec (inputs : Inputs (F p)) (out: KeccakState (F p)) : Prop :=
+  let ⟨state, d⟩ := inputs
+  let h_norm := ∀ i : Fin 25, out[i].is_normalized
+
+  let state_u64 := state.map (fun x => x.value)
+  let d_u64 := d.map (fun x => x.value)
+  let out_u64 := out.map (fun x => x.value)
+
+  let state' := Clean.Gadgets.Keccak256.theta_xor state_u64 d_u64
+
+  h_norm ∧ state' = out_u64
+
+theorem soundness : Soundness (F p) assumptions spec := by
+  intro i0 env state_var ⟨state, d⟩ h_input ⟨state_norm, d_norm⟩ h_holds
+  simp only [circuit_norm] at h_input
+  dsimp only [circuit_norm, theta_xor, Xor.circuit, Rotation64.circuit] at h_holds
+  simp only [circuit_norm, subcircuit_norm] at h_holds
+  dsimp only [Xor.assumptions, Xor.spec, Rotation64.assumptions, Rotation64.spec] at h_holds
+  simp [add_assoc, and_assoc, -Fin.val_zero, -Fin.val_one', -Fin.val_one, -Fin.val_two] at h_holds
+
+  simp at h_input
+  obtain ⟨h_state, h_d⟩ := h_input
+
+  have s_d (i : Fin 5) : eval env (state_var.d[i.val]) = d[i.val] := by
+    rw [← h_d, Vector.getElem_map]
+
+  have s_state (i : Fin 25) : eval env (state_var.state[i.val]) = state[i.val] := by
+    rw [← h_state, Vector.getElem_map]
+
+  simp only [s_d, s_state] at h_holds
+  simp [circuit_norm, spec, Clean.Gadgets.Keccak256.theta_xor, Clean.Gadgets.Keccak256.xor_u64, Fin.forall_fin_succ,
+    -Fin.val_zero, -Fin.val_one', -Fin.val_one, -Fin.val_two]
+
+  repeat
+    first
+    | obtain ⟨ h, h_holds ⟩ := h_holds
+    | let h := h_holds; let h_holds := True
+    specialize h (state_norm _) (d_norm _)
+    obtain ⟨ xor, norm ⟩ := h
+    simp [xor, norm]
+
+
+theorem completeness : Completeness (F p) KeccakState assumptions := by
+  intro i0 env state_var h_env state h_input h_assumptions
+  simp only [circuit_norm] at h_input
+  dsimp only [circuit_norm, theta_xor, Xor.circuit, Rotation64.circuit]
+  simp only [circuit_norm, subcircuit_norm]
+  dsimp only [Xor.assumptions, Xor.spec]
+  simp [add_assoc]
+  sorry
+
+def circuit : FormalCircuit (F p) Inputs KeccakState := {
+  elaborated with
+  assumptions
+  spec
+  soundness
+  completeness
+}
+
 end Gadgets.Keccak.ThetaXor
