Clean/Gadgets/Keccak/KeccakState.lean
@@ -1,6 +1,45 @@
 import Clean.Types.U64
 import Clean.Circuit.Provable
+import Clean.Utils.Field
 
 namespace Clean.Gadgets.Keccak256
 
+variable {p : ℕ} [Fact p.Prime]
+variable [p_large_enough: Fact (p > 512)]
+
 @[reducible] def KeccakState := ProvableVector U64 25
+
+
+@[reducible]
+def KeccakState_is_normalized_iff (state : KeccakState (F p)) :
+    (∀ i : Fin 25, state[i].is_normalized) ↔
+    state[0].is_normalized ∧
+    state[1].is_normalized ∧
+    state[2].is_normalized ∧
+    state[3].is_normalized ∧
+    state[4].is_normalized ∧
+    state[5].is_normalized ∧
+    state[6].is_normalized ∧
+    state[7].is_normalized ∧
+    state[8].is_normalized ∧
+    state[9].is_normalized ∧
+    state[10].is_normalized ∧
+    state[11].is_normalized ∧
+    state[12].is_normalized ∧
+    state[13].is_normalized ∧
+    state[14].is_normalized ∧
+    state[15].is_normalized ∧
+    state[16].is_normalized ∧
+    state[17].is_normalized ∧
+    state[18].is_normalized ∧
+    state[19].is_normalized ∧
+    state[20].is_normalized ∧
+    state[21].is_normalized ∧
+    state[22].is_normalized ∧
+    state[23].is_normalized ∧
+    state[24].is_normalized := by
+  simp only [Fin.getElem_fin, Fin.forall_fin_succ, Fin.isValue,
+    Fin.val_zero, Fin.val_succ, zero_add, Nat.reduceAdd, Fin.val_eq_zero, IsEmpty.forall_iff,
+    and_true]
+
+end Clean.Gadgets.Keccak256
